Finish a generalized version of truth lemma for Intuitionistic completeness.

PropositionalLogic/CanonicalKripke.v
@@ -22,41 +22,21 @@ Instance nL: NormalLanguage L := PropositionalLanguage.nL Var.
 Instance pL: PropositionalLanguage L := PropositionalLanguage.pL Var.
 Instance R: SyntacticReduction L := IntuitionisticReduction.
 Instance nR: NormalSyntacticReduction L R := PropositionalLanguage.nIntuitionisticReduction.
-Instance G: ProofTheory L := IntuitionisticPropositionalLogic.G Var.
-Instance nG: NormalProofTheory L G := IntuitionisticPropositionalLogic.nG Var.
-Instance mpG: MinimunPropositionalLogic L G := IntuitionisticPropositionalLogic.mpG Var.
-Instance icG: ReductionConsistentProofTheory IntuitionisticReduction G := IntuitionisticPropositionalLogic.icG Var.
-Instance ipG: IntuitionisticPropositionalLogic L G := IntuitionisticPropositionalLogic.ipG Var.
-Instance SM: Semantics L := KripkeSemantics_All.SM Var.
-Instance icSM: ReductionConsistentSemantics IntuitionisticReduction SM := KripkeSemantics_All.icSM Var.
 
-Definition DCS: Type := sig (fun Phi =>
+Definition DCS (Gamma: ProofTheory L): Type := sig (fun Phi =>
   derivable_closed Phi /\
   orp_witnessed Phi /\
   consistent Phi).
 
-Definition canonical_frame: KripkeSemantics.frame.
-  refine (KripkeSemantics.Build_frame DCS (fun a b => Included _ (proj1_sig b) (proj1_sig a)) _).
-  constructor.
-  + hnf; intros.
-    hnf; intros; auto.
-  + hnf; intros.
-    hnf; intros; auto.
-Defined.
+Record canonical (Gamma: ProofTheory L) {SM: Semantics L} {icSM: ReductionConsistentSemantics IntuitionisticReduction SM} {pkSM: PreKripkeSemantics L SM} {kiSM: KripkeIntuitionisticSemantics L SM} (M: Kmodel): Type := {
+  underlying_bij :> bijection (Kworlds M) (DCS Gamma);
+  canonical_relation: forall m n m' n',
+    bij_R _ _ underlying_bij m m' ->
+    bij_R _ _ underlying_bij n n' ->
+    (Korder m n <-> Included _ (proj1_sig n') (proj1_sig m'))
+}.
 
-Program Definition canonical_eval: Var -> KripkeSemantics.sem canonical_frame :=
-  fun p a => a (PropositionalLanguage.varp p).
-Next Obligation.
-  apply H; auto.
-Qed.
-
-Definition canonical_Kmodel: KripkeSemantics_All.Kmodel :=
-  KripkeSemantics_All.Build_Kmodel Var canonical_frame canonical_eval.
-
-Definition canonical_model (Phi: DCS): model :=
-  KripkeSemantics_All.Build_model Var canonical_Kmodel Phi.
-
-Lemma Lindenbaum_lemma:
+Lemma Lindenbaum_lemma {Gamma: ProofTheory L} {nGamma: NormalProofTheory L Gamma} {mpGamma: MinimunPropositionalLogic L Gamma} {icGamma: ReductionConsistentProofTheory IntuitionisticReduction Gamma} {ipGamma: IntuitionisticPropositionalLogic L Gamma}:
   forall Phi x,
     ~ Phi |-- x ->
     exists Psi,
@@ -140,94 +120,80 @@ Proof.
     auto.
 Qed.
 
-Lemma truth_lemma: forall (Phi: DCS) x, canonical_model Phi |= x <-> proj1_sig Phi x.
+Lemma truth_lemma {Gamma: ProofTheory L} {nGamma: NormalProofTheory L Gamma} {mpGamma: MinimunPropositionalLogic L Gamma} {icGamma: ReductionConsistentProofTheory IntuitionisticReduction Gamma} {ipGamma: IntuitionisticPropositionalLogic L Gamma} {SM: Semantics L} {icSM: ReductionConsistentSemantics IntuitionisticReduction SM} {pkSM: PreKripkeSemantics L SM} {kiSM: KripkeIntuitionisticSemantics L SM}:
+  forall M (X: canonical Gamma M),
+   (forall m Phi v,
+      bij_R _ _ X m Phi ->
+      (KRIPKE: M, m |= PropositionalLanguage.varp v <-> proj1_sig Phi (PropositionalLanguage.varp v))) ->
+   (forall m Phi,
+      bij_R _ _ X m Phi ->
+      forall x, KRIPKE: M, m |= x <-> proj1_sig Phi x).
 Proof.
   intros.
+  rename H into ATOM_ASSUM, H0 into H.
   revert x.
-  pose proof (fun Phi: DCS => derivable_closed_element_derivable (proj1_sig Phi) (proj1 (proj2_sig Phi))).
-  apply (truth_lemma_from_syntactic_reduction _ _ _ _ _ (H Phi)).
+  pose proof (fun Phi: DCS Gamma => derivable_closed_element_derivable (proj1_sig Phi) (proj1 (proj2_sig Phi))).
+  apply (truth_lemma_from_syntactic_reduction _ _ _ _ _ (H0 Phi)).
   intros.
-  revert Phi.
-  induction x; try solve [inversion H0]; intros.
-  + destruct H0.
-    specialize (IHx1 H0 Phi).
-    specialize (IHx2 H1 Phi).
+  revert Phi m H.
+  induction x; try solve [inversion H1]; intros.
+  + destruct H1.
+    specialize (IHx1 H1 Phi m H).
+    specialize (IHx2 H2 Phi m H).
     pose proof DCS_andp_iff (proj1_sig Phi) (proj1 (proj2_sig Phi)) x1 x2.
-    simpl in *.
-    unfold KripkeSemantics.sem_and.
+    change (PropositionalLanguage.andp x1 x2) with (x1 && x2).
+    rewrite sat_andp.
     tauto.
-  + destruct H0.
-    specialize (IHx1 H0 Phi).
-    specialize (IHx2 H1 Phi).
+  + destruct H1.
+    specialize (IHx1 H1 Phi m H).
+    specialize (IHx2 H2 Phi m H).
     pose proof DCS_orp_iff (proj1_sig Phi) (proj1 (proj2_sig Phi)) (proj1 (proj2 (proj2_sig Phi))) x1 x2.
     simpl in *.
-    unfold KripkeSemantics.sem_or.
+    change (PropositionalLanguage.orp x1 x2) with (x1 || x2).
+    rewrite sat_orp.
     tauto.
-  + destruct H0.
-    specialize (IHx1 H0).
-    specialize (IHx2 H1).
+  + destruct H1.
+    specialize (IHx1 H1).
+    specialize (IHx2 H2).
     split.
     - intros.
-      rewrite H.
-      apply (@deduction_theorem _ _ _ _ (IntuitionisticPropositionalLogic.mpG Var)).
+      rewrite H0.
+      change (PropositionalLanguage.impp x1 x2) with (x1 --> x2) in *.
+      apply deduction_theorem.
       apply Classical_Prop.NNPP; intro.
-      pose proof Lindenbaum_lemma _ _ H3.
-      destruct H4 as [Psi [? [? ?]]].
-      hnf in H2.
-      specialize (H2 (exist _ Psi H6)).
-      assert (Included _ (proj1_sig Phi) Psi) by (hnf; intros; apply H4; left; auto).
-      specialize (H2 H7).
-      simpl in IHx1, IHx2.
-      simpl in H2.
-      rewrite IHx1, IHx2 in H2; simpl in H2.
-      assert (Psi x1) by (apply H4; right; constructor).
-      specialize (H2 H8).
-      specialize (H (exist _ Psi H6) x2); simpl in H.
-      rewrite H in H2; auto.
+      pose proof Lindenbaum_lemma _ _ H4.
+      destruct H5 as [Psi' [? [? ?]]].
+      set (Psi := exist _ Psi' H7: DCS Gamma).
+      change Psi' with (proj1_sig Psi) in H5, H6.
+      clearbody Psi; clear Psi' H7.
+      rewrite sat_impp in H3.
+      destruct (su_bij _ _ X Psi) as [n ?].
+      specialize (H3 n).
+      assert (Included _ (proj1_sig Phi) (proj1_sig Psi)) by (hnf; intros; apply H5; left; auto).
+      rewrite <- canonical_relation in H8 by eauto.
+      specialize (H3 H8).
+      rewrite IHx1, IHx2 in H3 by eauto.
+      assert (proj1_sig Psi x1) by (apply H5; right; constructor).
+      specialize (H3 H9).
+      specialize (H0 Psi x2).
+      rewrite H0 in H3; auto.
     - intros.
-      hnf; intros Psi ?H.
-      change DCS in Psi.
-      simpl in H3.
-      simpl in IHx1, IHx2.
-      rewrite IHx1, IHx2.
+      change (PropositionalLanguage.impp x1 x2) with (x1 --> x2) in *.
+      rewrite sat_impp; intros n ?H.
+      destruct (im_bij _ _ X n) as [Psi ?].
+      rewrite IHx1, IHx2 by eauto.
       intros.
-      rewrite H in H2, H4 |- *.
-      eapply derivable_weaken in H2; [| exact H3].
-      eapply derivable_modus_ponens; [exact H4 | exact H2].
-  + simpl.
-    split; [intros [] | intros].
-    rewrite H in H1.
+      rewrite H0 in H3, H6 |- *.
+      rewrite canonical_relation in H4 by eauto.
+      eapply derivable_weaken in H3; [| exact H4].
+      eapply derivable_modus_ponens; [exact H6 | exact H3].
+  + pose proof sat_falsep M m.
+    split; [intros; tauto | intros].
+    rewrite H0 in H3.
     pose proof proj2_sig Phi.
-    destruct H2 as [_ [_ ?]].
-    apply H2; auto.
-  + simpl.
-    unfold canonical_model.
-    tauto.
-Qed.
-
-Theorem complete_intuitionistic_kripke: strongly_complete G SM.
-Proof.
-  assert (forall Phi x, ~ Phi |-- x -> ~ Phi |== x).
-  + intros.
-    assert (exists Psi: DCS, Included _ Phi (proj1_sig Psi) /\ ~ proj1_sig Psi |-- x).
-    Focus 1. {
-      apply Lindenbaum_lemma in H.
-      destruct H as [Psi [? [? ?]]].
-      exists (exist _ Psi H1).
-      simpl; auto.
-    } Unfocus.
-    destruct H0 as [Psi [? ?]].
-    intro.
-    specialize (H2 (canonical_model Psi)).
-    apply H1.
-    rewrite <- derivable_closed_element_derivable by (exact (proj1 (proj2_sig Psi))).
-    apply truth_lemma.
-    apply H2; intros.
-    apply truth_lemma.
-    apply H0; auto.
-  + hnf; intros.
-    apply Classical_Prop.NNPP; intro; revert H0.
-    apply H; auto.
+    destruct H4 as [_ [_ ?]].
+    exfalso; apply H4; auto.
+  + auto.
 Qed.
 
 End Completeness.
