PropositionalLogic/Classical2Intuitionistic.v
@@ -1,14 +1,15 @@
 Require Import Logic.LogicBase.
-Require Import Logic.SyntacticReduction.
+Require Import Logic.MinimunLogic.MinimunLogic.
+Require Import Logic.MinimunLogic.SyntacticReduction.
+Require Import Logic.MinimunLogic.ContextProperty.
 Require Import Logic.PropositionalLogic.Syntax.
-Require Import Logic.PropositionalLogic.MinimunPropositionalLogic.
 Require Import Logic.PropositionalLogic.ClassicalPropositionalLogic.
 Require Import Logic.PropositionalLogic.IntuitionisticPropositionalLogic.
 
 Local Open Scope logic_base.
 Local Open Scope PropositionalLogic.
 
-Definition ClassicalImpAndOrAsPrimeReduction {L: Language} {nL: NormalLanguage L} {pL: PropositionalLanguage L} {Gamma: ProofTheory L} {nGamma: NormalProofTheory L Gamma} {mpGamma: MinimunPropositionalLogic L Gamma} {rcGamma: ReductionConsistentProofTheory MendelsonReduction Gamma} {cpGamma: ClassicalPropositionalLogic L Gamma}:
+Definition ClassicalImpAndOrAsPrimeReduction {L: Language} {nL: NormalLanguage L} {pL: PropositionalLanguage L} {Gamma: ProofTheory L} {nGamma: NormalProofTheory L Gamma} {mpGamma: MinimunPropositionalLogic L Gamma} {mcGamma: ReductionConsistentProofTheory MendelsonReduction Gamma} {cpGamma: ClassicalPropositionalLogic L Gamma}:
   AtomicReductionConsistentProvable ImpAndOrAsPrime.atomic_reduce Gamma.
 Proof.
   hnf; intros.
@@ -36,7 +37,7 @@ Proof.
     apply double_negp_add.
 Qed.
 
-Definition ClassicalIffReduction {L: Language} {nL: NormalLanguage L} {pL: PropositionalLanguage L} {Gamma: ProofTheory L} {nGamma: NormalProofTheory L Gamma} {mpGamma: MinimunPropositionalLogic L Gamma} {rcGamma: ReductionConsistentProofTheory MendelsonReduction Gamma} {cpGamma: ClassicalPropositionalLogic L Gamma}:
+Definition ClassicalIffReduction {L: Language} {nL: NormalLanguage L} {pL: PropositionalLanguage L} {Gamma: ProofTheory L} {nGamma: NormalProofTheory L Gamma} {mpGamma: MinimunPropositionalLogic L Gamma} {mcGamma: ReductionConsistentProofTheory MendelsonReduction Gamma} {cpGamma: ClassicalPropositionalLogic L Gamma}:
   AtomicReductionConsistentProvable ReduceIff.atomic_reduce Gamma.
 Proof.
   hnf; intros.
@@ -49,7 +50,7 @@ Proof.
   + apply imp_refl.
 Qed.
 
-Definition ClassicalTrueReduction {L: Language} {nL: NormalLanguage L} {pL: PropositionalLanguage L} {Gamma: ProofTheory L} {nGamma: NormalProofTheory L Gamma} {mpGamma: MinimunPropositionalLogic L Gamma} {rcGamma: ReductionConsistentProofTheory MendelsonReduction Gamma} {cpGamma: ClassicalPropositionalLogic L Gamma}:
+Definition ClassicalTrueReduction {L: Language} {nL: NormalLanguage L} {pL: PropositionalLanguage L} {Gamma: ProofTheory L} {nGamma: NormalProofTheory L Gamma} {mpGamma: MinimunPropositionalLogic L Gamma} {mcGamma: ReductionConsistentProofTheory MendelsonReduction Gamma} {cpGamma: ClassicalPropositionalLogic L Gamma}:
   AtomicReductionConsistentProvable ReduceTrue.atomic_reduce Gamma.
 Proof.
   hnf; intros.
@@ -61,6 +62,42 @@ Proof.
     apply true_provable.
 Qed.
 
+Definition ClassicalPropositionalPropagationReduction {L: Language} {nL: NormalLanguage L} {pL: PropositionalLanguage L} {Gamma: ProofTheory L} {nGamma: NormalProofTheory L Gamma} {mpGamma: MinimunPropositionalLogic L Gamma} {mcGamma: ReductionConsistentProofTheory MendelsonReduction Gamma} {cpGamma: ClassicalPropositionalLogic L Gamma}:
+  PropositonalPropagationConsistentProvable Gamma.
+Proof.
+  hnf; intros.
+  destruct H; destruct H0.
+  + rewrite !imp1_propag_denote.
+Admitted.
+
+Module ClassicalPropositionalLogic2Intuitionistic.
+
+Context (Var: Type).
+
+Instance L: Language := PropositionalLanguage.L Var.
+Instance nL: NormalLanguage L := PropositionalLanguage.nL Var.
+Instance pL: PropositionalLanguage L := PropositionalLanguage.pL Var.
+Instance R: SyntacticReduction L := MendelsonReduction.
+Instance G: ProofTheory L := ClassicalPropositionalLogic.G Var.
+Instance nG: NormalProofTheory L G := ClassicalPropositionalLogic.nG Var.
+Instance mpG: MinimunPropositionalLogic L G := ClassicalPropositionalLogic.mpG Var.
+Instance mcG: ReductionConsistentProofTheory MendelsonReduction G := ClassicalPropositionalLogic.mcG Var.
+Instance cpG: ClassicalPropositionalLogic L G := ClassicalPropositionalLogic.cpG Var.
+
+Instance icG: ReductionConsistentProofTheory IntuitionisticReduction G.
+  apply Build3_ReductionConsistentProofTheory.
+  + simpl.
+    repeat apply disjunction_reduce_consistent_provable.
+    - apply ClassicalImpAndOrAsPrimeReduction.
+    - apply ClassicalIffReduction.
+    - apply ClassicalTrueReduction.
+  + apply PropositionalLanguage.RPPC_RPC.
+    apply ClassicalPropositionalPropagationReduction.
+Qed.
+
+Instance ipG: IntuitionisticPropositionalLogic L G.
+Admitted.
+(*
 Definition ClassicalIntuitionisticReduction {L: Language} {nL: NormalLanguage L} {pL: PropositionalLanguage L} {Gamma: ProofTheory L} {nGamma: NormalProofTheory L Gamma} {mpGamma: MinimunPropositionalLogic L Gamma} {rcGamma: ReductionConsistentProofTheory MendelsonReduction Gamma} {cpGamma: ClassicalPropositionalLogic L Gamma}:
   ReductionConsistentProofTheory IntuitionisticReduction Gamma.
 Proof.
@@ -74,3 +111,5 @@ Proof.
     destruct sp; simpl.
 Abort.
 
+*)
+End ClassicalPropositionalLogic2Intuitionistic.
